coq/DSigmaHCOL/TypeSig.v
@@ -1,0 +1,157 @@
+Require Import Coq.Arith.Arith.
+Require Import Coq.Structures.OrderedTypeEx.
+Require Import Coq.Arith.PeanoNat.
+Require Import Coq.Arith.Peano_dec.
+Require Import Coq.Logic.Decidable.
+Require Import Omega.
+Require Import Psatz.
+
+Require Import CoLoR.Util.Nat.NatUtil.
+
+From Coq.FSets Require Import
+     FSetAVL
+     FSetInterface
+     FSetFacts
+     FSetProperties
+     FSetToFiniteSet
+     FMapAVL
+     FMapInterface
+     FMapFacts.
+
+Require Import Helix.HCOL.CarrierType.
+
+Require Import Helix.DSigmaHCOL.DSigmaHCOL.
+Require Import Helix.DSigmaHCOL.DSigmaHCOLEval.
+
+Require Import MathClasses.misc.util.
+Require Import MathClasses.interfaces.canonical_names.
+Require Import MathClasses.orders.minmax MathClasses.interfaces.orders.
+Require Import MathClasses.implementations.peano_naturals.
+Require Import MathClasses.orders.orders.
+Require Import MathClasses.misc.decision.
+
+Require Import Helix.Util.OptionSetoid.
+Require Import Helix.Tactics.HelixTactics.
+
+Open Scope list_scope.
+
+Require Import ExtLib.Structures.Monads.
+Require Import ExtLib.Data.Monads.OptionMonad.
+
+Import MonadNotation.
+Local Open Scope monad_scope.
+Local Open Scope nat_scope.
+
+Module TM := FMapAVL.Make(Nat_as_OT).
+Module Import TP := FMapFacts.WProperties_fun(Nat_as_OT)(TM).
+(* [TypeSig] is a signature of an evaluation context, which maps
+   De-Brujn indices to expected types *)
+Definition TypeSig := TM.t DSHType.
+
+Global Instance DSHValType_Decision (v:DSHVal) (t:DSHType):
+  Decision (DSHValType v t).
+Proof.
+  unfold decidable.
+  destruct v,t; try (left;constructor); right; intros H; inversion H.
+Qed.
+
+Definition DSHValType_bool (v:DSHVal) (t:DSHType) := bool_decide (DSHValType v t).
+
+(* True if nth context element has expected type. decidable. *)
+Definition contextEnsureType (σ: evalContext) (k:nat) (t:DSHType) : Prop :=
+  match nth_error σ k with
+  | Some v => DSHValType v t
+  | _ => False
+  end.
+
+Global Instance contextEnsureType_Decision {σ k t}:
+  Decision (contextEnsureType σ k t).
+Proof.
+  unfold Decision, contextEnsureType.
+  break_match; auto.
+  apply DSHValType_Decision.
+Qed.
+
+Definition typecheck_env (tm:TypeSig) (σ: evalContext) :  Prop :=
+  forall k t, TM.MapsTo k t tm -> contextEnsureType σ k t.
+
+Global Instance typecheck_env_Decision (tm:TypeSig) (σ: evalContext):
+  Decision (typecheck_env tm σ).
+Proof.
+Admitted.
+
+(* alternative definition on booleans using `for_all` *)
+Definition typecheck_env_bool (tm:TypeSig) (σ: evalContext) : bool :=
+  TP.for_all (fun k t => bool_decide (contextEnsureType σ k t)) tm.
+
+(* Sanity check *)
+Lemma typecheck_env_bool_iff (tm:TypeSig) (σ: evalContext):
+  bool_decide (typecheck_env tm σ) ≡ typecheck_env_bool tm σ.
+Proof.
+Admitted.
+
+Definition TypeSigMExpr (me:MExpr) : TypeSig :=
+  match me with
+  | MVar v => TM.add v DSHMemBlock (TM.empty _)
+  | MConst _ => TM.empty _
+  end.
+
+
+Definition TypeSigUnion := TP.update (elt:=DSHType).
+
+
+(* True, if given type signatures do not have conflicts.
+   A conflict occurs when different values occur at
+   different signatures at the same index.
+ *)
+Definition TypeSigCompat (s1 s2:TypeSig) : Prop. Admitted.
+
+Fixpoint TypeSigNExpr (ne:NExpr) : TypeSig :=
+  match ne with
+  | NVar v => TM.add v DSHnat (TM.empty _)
+  | NConst x => TM.empty _
+  | NDiv a b => TypeSigUnion (TypeSigNExpr a) (TypeSigNExpr b)
+  | NMod a b => TypeSigUnion (TypeSigNExpr a) (TypeSigNExpr b)
+  | NPlus a b => TypeSigUnion (TypeSigNExpr a) (TypeSigNExpr b)
+  | NMinus a b => TypeSigUnion (TypeSigNExpr a) (TypeSigNExpr b)
+  | NMult a b => TypeSigUnion (TypeSigNExpr a) (TypeSigNExpr b)
+  | NMin a b => TypeSigUnion (TypeSigNExpr a) (TypeSigNExpr b)
+  | NMax a b => TypeSigUnion (TypeSigNExpr a) (TypeSigNExpr b)
+  end.
+
+Fixpoint TypeSigAExpr (ae:AExpr) : TypeSig :=
+  match ae with
+  | AVar v => TM.add v DSHCarrierA (TM.empty _)
+  | AConst _ => TM.empty _
+  | ANth m n => TypeSigUnion (TypeSigMExpr m) (TypeSigNExpr n)
+  | AAbs a => TypeSigAExpr a
+  | APlus a b => TypeSigUnion (TypeSigAExpr a) (TypeSigAExpr b)
+  | AMinus a b => TypeSigUnion (TypeSigAExpr a) (TypeSigAExpr b)
+  | AMult a b => TypeSigUnion (TypeSigAExpr a) (TypeSigAExpr b)
+  | AMin a b => TypeSigUnion (TypeSigAExpr a) (TypeSigAExpr b)
+  | AMax a b => TypeSigUnion (TypeSigAExpr a) (TypeSigAExpr b)
+  | AZless a b => TypeSigUnion (TypeSigAExpr a) (TypeSigAExpr b)
+  end.
+
+
+(* make sure 2 contexts are quivalent at locations from given [TypeSig].
+   additionally makes typechecks both contexts wrt [TypeSig] *)
+Definition context_equiv_at_TypeSig (tm:TypeSig) : relation evalContext
+  := fun σ0 σ1 =>
+       forall k t, TM.MapsTo k t tm ->
+              contextEnsureType σ0 k t /\
+              contextEnsureType σ1 k t /\
+              context_lookup σ0 k = context_lookup σ1 k.
+
+Definition TypeSigAExpr_UnCarrierA (f: DSHIBinCarrierA) : TypeSig := TypeSigAExpr f.
+Definition TypeSigAExpr_IUnCarrierA (f: DSHIBinCarrierA) : TypeSig := TypeSigAExpr f.
+Definition TypeSigAExpr_BinCarrierA (f: DSHBinCarrierA) : TypeSig := TypeSigAExpr f.
+Definition TypeSigAExpr_IBinCarrierA (f: DSHIBinCarrierA) : TypeSig := TypeSigAExpr f.
+
+
+Lemma context_equiv_at_TypeSig_widening {σ0 σ1 tm foo0 foo1}:
+  context_equiv_at_TypeSig tm σ0 σ1 ->
+  context_equiv_at_TypeSig tm (foo0 :: σ0) (foo1 :: σ1).
+Proof.
+  intros H.
+Admitted.
